Removed CountM. Improved the Section handling.
Signed-off-by: Andrew Miller <amiller@dappervision.com>

coq/monads_.v
@@ -1,20 +1,32 @@
 Require Import monads.
+Require Import canonical_names.
+
+(* Identity Monad *)
 
 Definition IdM : Type -> Type := fun A => A.
 Definition IdM_Return : MonadReturn IdM := fun A a => a.
 Definition IdM_Bind : MonadBind IdM := fun A B ma f => f ma.
 
+(* TODO *)
+(* Prove monad laws? *)
 Instance IdentityMonad : Monad IdM (H:=IdM_Return) (H0:=IdM_Bind). 
 admit. Defined.
 
-Definition StateM S : Type -> Type := fun A => S -> prod S A.
-Definition StateM_Return {S} : MonadReturn (StateM S) := fun A a s => (s, a).
-Definition StateM_Bind {S} : MonadBind (StateM S) := fun A B m f r =>
+
+(* State Monad *)
+Section State.
+Context (S : Type).
+Context (S_equiv : Equiv S).
+
+Definition StateM : Type -> Type := fun A => S -> prod S A.
+Definition StateM_Return : MonadReturn StateM := fun A a s => (s, a).
+Definition StateM_Bind : MonadBind StateM := fun A B m f r =>
   match m r with (s, a) => (f a) s end.
-
-Definition CountM := StateM nat.
-Definition CountM_Me : forall A : Type, canonical_names.Equiv A -> 
-   canonical_names.Equiv (CountM A). admit. Defined.
-
-Instance CountMonad : Monad CountM (Me:=CountM_Me) (H:=StateM_Return) (H0:=StateM_Bind).
+Definition StateM_Me: forall A : Type, Equiv A -> Equiv (StateM A). 
 admit. Defined.
+
+(* TODO *)
+(* Prove monad laws? *)
+Instance StateMonad : Monad StateM (Me:=StateM_Me) (H:=StateM_Return) (H0:=StateM_Bind).
+admit. Defined.
+End State.
