coq/merkle.v
@@ -16,7 +16,6 @@ Require Import monads_.
    hash functions from this HDomain. This allows us to express Collisions
   very generally. *)
 
-Context (HRange : Set).
 
 (* Define a type of functional maps. *)
 (* TODO: Instantiate this by borrowing from FMap.FMapInterfaces Sord*)
@@ -28,48 +27,46 @@ Parameter search : Map -> k -> option v.
 Parameter insert : Map -> k -> v -> Map.
 Parameter delete : Map -> k -> Map.
 
+Section WithRange.
+Variable HRange : Set.
+
 Section WithDomain.
 (* Introduce a Domain for a hash function, as well as an instance
    from Domain to Range. Define a Collision of two distinct elements
    from the Domain with the same image in Range. *)
-Context (HDomain : Set).
-Context (h : HDomain -> HRange).
+Variables HDomain : Set.
+Variables h : HDomain -> HRange.
 
 Definition Collision := {ab | match ab with (a, b) => 
                          a <> b /\ h a = h b end}.
 
-(* Define a family of Monads in which a computation 'hash' is 
-   defined. We provide two instances of this family. *)
+(* Define a family of monadic hash computations. We will provide
+   two instances of this family, each for a specific monad. *)
 Class HashComputation `{M0:Monad M} :=
   hash_computation : HDomain -> M HRange.
 
-(* The first instance is an identity monad, and the computation 
-   simply evaluates the hash function and returns the result. This
-   is suitable for a correctness proof. *)
+(* The first instance of HashComputation runs in the identity monad.
+   The computation simply evaluates the hash function and returns 
+   the result. The monad scaffolding falls away, which is desirable
+   for correctness proofs. *)
 Instance HashIdC : HashComputation (M0:=IdentityMonad) := 
   { hash_computation d := h d }.
 
-(* The second instance includes a counter, and the hash computation
-   increments the counter every time. *)
-Instance HashCountC : HashComputation (M0:=CountMonad) :=
+(* The second instance runs in a Counter monad (i.e., StateM nat). 
+   The computation evaluates the hash and returns it, but it also
+   increments the counter. For a worst-case complexity proof of 
+   a computation, it will suffice to bound the size of the counter
+   after the computation completes. *)
+Instance HashCountC : HashComputation (M0:=StateMonad nat) :=
   { hash_computation d := fun c => (S c, h d) }.
 
-(* A computation defined for the entire family of HashMonads can only
-   be constructed by composing hash_computations using (return) and (>>=).
-*)
-Definition HashMonadComputation A := forall M `{Monad M} `{HashComputation}, M A.
+
 
 (*- Define a MerkleInstance type containing several sets 
     and a handful of computations *)
-Class MerkleData := {
-  Tree : Set;
-  VO : Set;
-  Digest : Set;
-  Empty : Tree
-}.
 
 (* The computations must be defined for all Monads supporting a hash computation *)
-Class Computations M `{MerkleData} := {
+Class Computations M Digest VO Tree := {
     digest_c : Tree -> M Digest;
     search_c : Tree -> k -> M VO;
     insert_c : Tree -> k -> v -> M (prod VO Tree);
@@ -84,15 +81,20 @@ Class Computations M `{MerkleData} := {
     delete_f : Digest -> k -> VO -> VO -> M (option Collision)
 }.
 
-Class MerkleInstance := {
-   MD : MerkleData;
+
+Class MerkleComputations := {
+   Digest : Set;
+   VO : Set;
+   Tree : Set;
+   Empty : Tree;
 
    (* The computations must be defined over all monads with 
-      an available HashComputation, (not just the h in our scope) *)
-   CC : forall M `{HC:HashComputation}, Computations M;
+      an available HashComputation *)
+   CC : forall M `{M0:Monad M} `{HC:HashComputation}, Computations M Digest VO Tree;
 
-   CCM := CC IdM (HC:=HashIdC);
-   CCC := CC CountM (HC:=HashCountC);
+   CCM := CC IdM (M0:=IdentityMonad) (HC:=HashIdC);
+   CountM := StateM nat;
+   CCC := CC CountM (M0:=StateMonad nat) (HC:=HashCountC);
 
 (* Requirement #1: Correctness *)
 (* Define a mapping from Trees to Maps. This is a homomorphism 
@@ -106,24 +108,23 @@ Class MerkleInstance := {
    T : Tree -> Map;
    T_empty : T Empty = empty;
 
+   digest : Tree -> Digest := fun t => digest_c (M:=IdM) t;
 
-   digest : Tree -> Digest := fun t => digest_c t;
-  
    search_T : forall t k, match search_c (M:=IdM) t k
               with vo =>
-                 search_v (digest t) k vo = Some (search (T t) k)
+                 search_v (M:=IdM) (digest t) k vo = Some (search (T t) k)
               end;
 
    insert_T : forall t k v, match insert_c (M:=IdM) t k v
               with (vo, t') => 
                  T t' = insert (T t) k v
-              /\ insert_v (digest t) k v vo = Some (digest t')
+              /\ insert_v (M:=IdM) (digest t) k v vo = Some (digest t')
               end;
 
    delete_T : forall t k, match delete_c (M:=IdM) t k
               with (vo, t') =>
                   T t' = delete (T t) k
-               /\ delete_v (digest t) k vo = Some (digest t')
+               /\ delete_v (M:=IdM) (digest t) k vo = Some (digest t')
               end;
 
 (* Requirement #2. Security *)
@@ -150,7 +151,6 @@ Class MerkleInstance := {
                    /\ delete_v (M:=IdM) d k vo' = Some r' ->
                       exists cc, delete_f (M:=IdM) d k vo vo' = Some cc;
 
-
 (* Requirement #3. Complexity *)
 (* All of the computations must run in O(poly N) time. When each
    computation is run under the Count monad, the number of accesses
@@ -159,18 +159,19 @@ Class MerkleInstance := {
 
    polybound : nat -> nat;
 
-   search_c_C : forall t k, match search_c (M:=CountM) t k 0
+   search_c_C : forall t k, match search_c (M:=StateM nat) t k 0
                      with (c, _) => c <= polybound (size (T t)) end;
-   insert_c_C : forall t k v, match insert_c (M:=CountM) t k v 0
+   insert_c_C : forall t k v, match insert_c (M:=StateM nat) t k v 0
                      with (c, _) => c <= polybound (size (T t)) end;
-   delete_c_C : forall t k, match delete_c (M:=CountM) t k 0
+   delete_c_C : forall t k, match delete_c (M:=StateM nat) t k 0
                      with (c, _) => c <= polybound (size (T t)) end
 }.
-
 End WithDomain.
 
-Class MerkleSolution := {
+Class MerkleInstance := {
    HDomain : Set;
-   MI : forall h : HDomain -> HRange, MerkleInstance HDomain h
+   MI : forall h : HDomain -> HRange, MerkleComputations HDomain h
 }.
+End WithRange.
 
+Definition MerkleSolution := forall HRange, MerkleInstance HRange.
